added skeleton for schmidt decomp.
Missing SVD, and 2 simpler helper lemmas.

Vectors.v
@@ -1,16 +1,10 @@
 Require Import QuantumLib.Matrix.
 Require Import QuantumLib.Quantum.
 Require Import QuantumLib.VectorStates.
+Require Import QuantumLib.Eigenvectors.
 From Proof Require Import QubitHelpers.
-
-Lemma a14 : forall (psi : Vector 4), 
-WF_Matrix psi -> ⟨ psi , psi ⟩ = 1 -> 
-exists (beta beta_p gamma gamma_p: Vector 2) (r : R)
-(* (WF_b : WF_Matrix beta) (WF_bp : WF_Matrix beta_p) (WF_g: WF_Matrix gamma) (WF_gp : WF_Matrix gamma_p) *),
-⟨ beta , beta_p ⟩ = 0 /\ ⟨ gamma , gamma_p ⟩ = 0 /\
-psi = √ (r) .* (beta ⊗ gamma) .+ √ (1-r) .* (beta_p ⊗ gamma_p).
-intros.
-Admitted.
+From Proof Require Import MatrixHelpers.
+From Proof Require Import AlgebraHelpers.
 
 (* Definition of lemma from old file Multiqubit*)
 Lemma qubit_decomposition2 : forall (phi : Vector 4), 
@@ -20,11 +14,216 @@ Proof.
   intros.
   exists (phi 0 0)%nat, (phi 1 0)%nat, (phi 2 0)%nat, (phi 3 0)%nat.
   lma'.
-  apply WF_plus. apply WF_plus. apply WF_plus.
-  apply WF_scale. apply WF_kron. reflexivity. reflexivity. apply WF_qubit0. apply WF_qubit0.
-  apply WF_scale. apply WF_kron. reflexivity. reflexivity. apply WF_qubit0. apply WF_qubit1.
-  apply WF_scale. apply WF_kron. reflexivity. reflexivity. apply WF_qubit1. apply WF_qubit0.
-  apply WF_scale. apply WF_kron. reflexivity. reflexivity. apply WF_qubit1. apply WF_qubit1.
+  solve_WF_matrix.
+Qed.
+
+Definition WF_Nonnegative {m n} (A : Matrix m n) :=
+WF_Matrix A /\ forall (i j: nat), Re (A i j) >= 0 /\ Im (A i j) = 0.
+
+Lemma SVD_2: forall (A : Square 2), 
+exists (U L V: Square 2), 
+WF_Unitary U /\ WF_Unitary V /\ WF_Diagonal L /\ WF_Nonnegative L /\ A = U × L × V.
+Proof. 
+Admitted.
+
+Lemma amplitudes_of_unit {n}: forall (a b : C) (u v w: Vector n), 
+u = a .* v .+ b .* w -> ⟨ u , u ⟩ = C1 -> ⟨ v , v ⟩ = C1 -> ⟨ w , w ⟩ = C1 -> 
+a^2 + b^2 = C1.
+Proof.
+Admitted.
+
+Lemma kron_inner_prod {n}: forall (u v: Vector n), 
+⟨ u ⊗ v, u ⊗ v ⟩ = ⟨ u, u ⟩ * ⟨ v, v ⟩.
+Proof. 
+Admitted.
+
+
+Lemma a14 : forall (psi : Vector 4), 
+WF_Matrix psi -> ⟨ psi , psi ⟩ = 1 -> 
+exists (beta beta_p gamma gamma_p: Vector 2) (r : R)
+(* (WF_b : WF_Matrix beta) (WF_bp : WF_Matrix beta_p) (WF_g: WF_Matrix gamma) (WF_gp : WF_Matrix gamma_p) *),
+⟨ beta , beta_p ⟩ = 0 /\ ⟨ gamma , gamma_p ⟩ = 0 /\
+psi = √ (r) .* (beta ⊗ gamma) .+ √ (1-r) .* (beta_p ⊗ gamma_p).
+intros psi WF_psi psi_unit_vector.
+assert (psi_decomp: psi = (psi 0 0)%nat .* ∣0,0⟩ .+ (psi 1 0)%nat .* ∣0,1⟩ .+ (psi 2 0)%nat .* ∣1,0⟩ .+ (psi 3 0)%nat .* ∣1,1⟩).
+{
+  lma'. solve_WF_matrix.
+}
+set (A := (fun x y =>
+match (x,y) with
+| (0,0) => (psi 0 0)%nat
+| (0,1) => (psi 1 0)%nat
+| (1,0) => (psi 2 0)%nat
+| (1,1) => (psi 3 0)%nat
+| _ => C0
+end) : (Square 2)).
+assert (exists_svd_A: exists (U L V: Square 2), WF_Unitary U /\ WF_Unitary V /\ WF_Diagonal L /\ WF_Nonnegative L /\ A = U × L × V). apply SVD_2.
+destruct exists_svd_A as [U [L [V [unitary_U [unitary_V [diag_L [nonneg_L A_decomp]]]]]]].
+assert (A_elem_decomp: forall (j k: nat), A j k = U j 0%nat * L 0%nat 0%nat * V 0%nat k + U j 1%nat * L 1%nat 1%nat * V 1%nat k).
+{
+  intros.
+  rewrite A_decomp.
+  unfold Mmult. simpl. Csimpl.
+  destruct diag_L as [WF_L ndiag_0_L].
+  assert (L10_0: L 1%nat 0%nat = 0). apply ndiag_0_L. lia.
+  assert (L01_0: L 0%nat 1%nat = 0). apply ndiag_0_L. lia.
+  rewrite L10_0. rewrite L01_0. Csimpl.
+  reflexivity.
+}
+assert (psi_alt: psi = (U 0%nat 0%nat * L 0%nat 0%nat * V 0%nat 0%nat +
+U 0%nat 1%nat * L 1%nat 1%nat * V 1%nat 0%nat) .* ∣ 0, 0 ⟩ .+ (U 0%nat 0%nat * L 0%nat 0%nat * V 0%nat 1%nat +
+U 0%nat 1%nat * L 1%nat 1%nat * V 1%nat 1%nat) .* ∣ 0, 1 ⟩
+.+ (U 1%nat 0%nat * L 0%nat 0%nat * V 0%nat 0%nat +
+U 1%nat 1%nat * L 1%nat 1%nat * V 1%nat 0%nat) .* ∣ 1, 0 ⟩ .+ 
+(U 1%nat 0%nat * L 0%nat 0%nat * V 0%nat 1%nat +
+U 1%nat 1%nat * L 1%nat 1%nat * V 1%nat 1%nat) .* ∣ 1, 1 ⟩).
+{
+  assert (psi_0: (U 0%nat 0%nat * L 0%nat 0%nat * V 0%nat 0%nat +
+  U 0%nat 1%nat * L 1%nat 1%nat * V 1%nat 0%nat) = psi 0%nat 0%nat). rewrite <- A_elem_decomp. unfold A. reflexivity.
+  assert (psi_1: (U 0%nat 0%nat * L 0%nat 0%nat * V 0%nat 1%nat +
+  U 0%nat 1%nat * L 1%nat 1%nat * V 1%nat 1%nat) = psi 1%nat 0%nat). rewrite <- A_elem_decomp. unfold A. reflexivity.
+  assert (psi_2: (U 1%nat 0%nat * L 0%nat 0%nat * V 0%nat 0%nat +
+  U 1%nat 1%nat * L 1%nat 1%nat * V 1%nat 0%nat) = psi 2%nat 0%nat). rewrite <- A_elem_decomp. unfold A. reflexivity.
+  assert (psi_3: (U 1%nat 0%nat * L 0%nat 0%nat * V 0%nat 1%nat +
+  U 1%nat 1%nat * L 1%nat 1%nat * V 1%nat 1%nat) = psi 3%nat 0%nat). rewrite <- A_elem_decomp. unfold A. reflexivity.
+  rewrite psi_0. rewrite psi_1. rewrite psi_2. rewrite psi_3.
+  apply psi_decomp.
+}
+assert (tensor_decomp: psi = L 0%nat 0%nat .* ((U 0%nat 0%nat .* ∣0⟩ .+ U 1%nat 0%nat .* ∣1⟩) ⊗ (V 0%nat 0%nat .* ∣0⟩ .+ V 0%nat 1%nat .* ∣1⟩))
+.+ L 1%nat 1%nat .* ((U 0%nat 1%nat .* ∣0⟩ .+ U 1%nat 1%nat .* ∣1⟩) ⊗ (V 1%nat 0%nat .* ∣0⟩ .+ V 1%nat 1%nat .* ∣1⟩))).
+{
+  rewrite psi_alt. lma'.
+  solve_WF_matrix. solve_WF_matrix.
+}
+set (beta := (U 0%nat 0%nat .* ∣0⟩ .+ U 1%nat 0%nat .* ∣1⟩)).
+set (gamma := (V 0%nat 0%nat .* ∣0⟩ .+ V 0%nat 1%nat .* ∣1⟩)).
+set (beta_p := (U 0%nat 1%nat .* ∣0⟩ .+ U 1%nat 1%nat .* ∣1⟩)).
+set (gamma_p := (V 1%nat 0%nat .* ∣0⟩ .+ V 1%nat 1%nat .* ∣1⟩)).
+set (r := ((Re (L 0%nat 0%nat))^2)%R).
+exists beta,beta_p,gamma,gamma_p,r.
+split. 2: split.
+unfold beta, beta_p.
+2: unfold gamma, gamma_p.
+1,2: rewrite inner_product_plus_l. 
+1,2: do 2 rewrite inner_product_plus_r.
+1,2: repeat rewrite inner_product_scale_l.
+1,2: repeat rewrite inner_product_scale_r.
+1,2: unfold inner_product.
+1,2: rewrite Mmult00, Mmult01, Mmult10, Mmult11. 
+1,2: Csimpl.
+destruct unitary_U as [WF_U U_unit_prop].
+assert (mat_element_decomp: (U 0%nat 0%nat) ^* * U 0%nat 1%nat + (U 1%nat 0%nat) ^* * U 1%nat 1%nat = 
+((U) † × U) 0%nat 1%nat). lca.
+rewrite mat_element_decomp. rewrite U_unit_prop. lca.
+apply transpose_unitary in unitary_V.
+destruct unitary_V as [WF_Vdag Vdag_unit_prop].
+rewrite adjoint_involutive in Vdag_unit_prop.
+assert (mat_element_decomp: (V 0%nat 0%nat) ^* * V 1%nat 0%nat + (V 0%nat 1%nat) ^* * V 1%nat 1%nat = 
+(V × (V) †) 1%nat 0%nat). lca.
+rewrite mat_element_decomp. rewrite Vdag_unit_prop. lca.
+assert (unit_coefs: (L 0%nat 0%nat)^2 + (L 1%nat 1%nat)^2 = 1).
+{
+  set (v := (U 0%nat 0%nat .* ∣0⟩ .+ U 1%nat 0%nat .* ∣1⟩) ⊗ (V 0%nat 0%nat .* ∣0⟩ .+ V 0%nat 1%nat .* ∣1⟩) : Vector 4).
+  fold v in tensor_decomp.
+  set (w := (U 0%nat 1%nat .* ∣0⟩ .+ U 1%nat 1%nat .* ∣1⟩) ⊗ (V 1%nat 0%nat .* ∣0⟩ .+ V 1%nat 1%nat .* ∣1⟩) : Vector 4).
+  fold w in tensor_decomp.
+  apply (amplitudes_of_unit (L 0%nat 0%nat) (L 1%nat 1%nat) psi v w).
+  apply tensor_decomp.
+  apply psi_unit_vector.
+  unfold v.
+  set (a := (U 0%nat 0%nat .* ∣0⟩ .+ U 1%nat 0%nat .* ∣1⟩)).
+  set (b := (V 0%nat 0%nat .* ∣0⟩ .+ V 0%nat 1%nat .* ∣1⟩)).
+  assert (temp: ⟨ a ⊗ b, a ⊗ b ⟩ = ⟨a, a⟩ * ⟨b, b⟩). apply kron_inner_prod.
+  rewrite temp at 1. clear temp.
+  unfold a,b.
+  repeat rewrite inner_product_plus_l. repeat rewrite inner_product_plus_r.
+  repeat rewrite inner_product_scale_l. repeat rewrite inner_product_scale_r.
+  unfold inner_product.
+  rewrite Mmult00, Mmult01, Mmult10, Mmult11. Csimpl.
+  assert (U_norm_helper: ((U 0%nat 0%nat) ^* * U 0%nat 0%nat + (U 1%nat 0%nat) ^* * U 1%nat 0%nat) = ((U) † × U) 0%nat 0%nat). lca.
+  assert (V_norm_helper: ((V 0%nat 0%nat) ^* * V 0%nat 0%nat + (V 0%nat 1%nat) ^* * V 0%nat 1%nat) = (V × (V) †) 0%nat 0%nat). lca.
+  rewrite U_norm_helper, V_norm_helper. clear U_norm_helper V_norm_helper.
+  destruct unitary_U as [_ unit_prop_U]. rewrite unit_prop_U.
+  apply transpose_unitary in unitary_V. destruct unitary_V as [_ unit_prop_Vadj]. rewrite adjoint_involutive in unit_prop_Vadj.
+  rewrite unit_prop_Vadj. lca.
+  unfold w.
+  set (a := (U 0%nat 1%nat .* ∣0⟩ .+ U 1%nat 1%nat .* ∣1⟩)).
+  set (b := (V 1%nat 0%nat .* ∣0⟩ .+ V 1%nat 1%nat .* ∣1⟩)).
+  assert (temp: ⟨ a ⊗ b, a ⊗ b ⟩ = ⟨a, a⟩ * ⟨b, b⟩). apply kron_inner_prod.
+  rewrite temp at 1. clear temp.
+  unfold a,b.
+  repeat rewrite inner_product_plus_l. repeat rewrite inner_product_plus_r.
+  repeat rewrite inner_product_scale_l. repeat rewrite inner_product_scale_r.
+  unfold inner_product.
+  rewrite Mmult00, Mmult01, Mmult10, Mmult11. Csimpl.
+  assert (U_norm_helper: ((U 0%nat 1%nat) ^* * U 0%nat 1%nat + (U 1%nat 1%nat) ^* * U 1%nat 1%nat) = ((U) † × U) 1%nat 1%nat). lca.
+  assert (V_norm_helper: ((V 1%nat 0%nat) ^* * V 1%nat 0%nat + (V 1%nat 1%nat) ^* * V 1%nat 1%nat) = (V × (V) †) 1%nat 1%nat). lca.
+  rewrite U_norm_helper, V_norm_helper. clear U_norm_helper V_norm_helper.
+  destruct unitary_U as [_ unit_prop_U]. rewrite unit_prop_U.
+  apply transpose_unitary in unitary_V. destruct unitary_V as [_ unit_prop_Vadj]. rewrite adjoint_involutive in unit_prop_Vadj.
+  rewrite unit_prop_Vadj. lca.
+}
+assert (first_coef: RtoC (√ r) = L 0%nat 0%nat).
+{
+  unfold r, RtoC.
+  apply c_proj_eq. unfold fst at 1.
+  assert (help: √ (Re (L 0%nat 0%nat) ^ 2) = Re (L 0%nat 0%nat)).
+  {
+    destruct nonneg_L as [_ nonneg_L_elem].
+    rewrite <- pow2_sqrt.
+    apply sqrt_pow.
+    all: apply Rge_le.
+    all: apply nonneg_L_elem.
+  }
+  rewrite help. clear help. unfold Re. reflexivity.
+  unfold snd at 1. destruct nonneg_L as [_ nonneg_L_elem].
+  unfold Im in nonneg_L_elem.
+  symmetry.
+  apply nonneg_L_elem.
+}
+assert (second_coef: RtoC (√ (1 - r)) = L 1%nat 1%nat).
+{
+  unfold r, RtoC.
+  apply c_proj_eq.
+  unfold fst at 1.
+  assert (r_unit_coefs: (Re (L 0%nat 0%nat) ^ 2 + Re (L 1%nat 1%nat)^ 2 = 1)%R).
+  {
+    destruct nonneg_L as [_ nonneg_L_elem]. unfold Im in nonneg_L_elem.
+    assert (L00_r: snd (L 0%nat 0%nat) = 0). apply nonneg_L_elem.
+    assert (L11_r: snd (L 1%nat 1%nat) = 0). apply nonneg_L_elem.
+    revert unit_coefs.
+    unfold RtoC, Re, Cpow, Cmult. simpl.
+    repeat rewrite L00_r. repeat rewrite L11_r. 
+    repeat rewrite Rmult_0_r. repeat rewrite Rmult_0_l.
+    repeat rewrite Rminus_0_r. repeat rewrite Rplus_0_r.
+    repeat rewrite Rmult_1_r. repeat rewrite Rmult_0_r.
+    intros unit_coefs. apply complex_split in unit_coefs.
+    destruct unit_coefs as [unit_coefs _].
+    revert unit_coefs. unfold Cplus. simpl.
+    trivial.
+  }
+  assert (r_unit_restate: (1 - Re (L 0%nat 0%nat) ^ 2 =Re (L 1%nat 1%nat) ^ 2)%R). 
+  {
+    rewrite <- r_unit_coefs.
+    lra. 
+  }
+  rewrite r_unit_restate.
+  assert (help: √ (Re (L 1%nat 1%nat) ^ 2) = Re (L 1%nat 1%nat)).
+  {
+    destruct nonneg_L as [_ nonneg_L_elem].
+    rewrite <- pow2_sqrt.
+    apply sqrt_pow.
+    all: apply Rge_le.
+    all: apply nonneg_L_elem.
+  }
+  rewrite help. clear help. unfold Re. reflexivity.
+  unfold snd at 1. destruct nonneg_L as [_ nonneg_L_elem].
+  unfold Im in nonneg_L_elem.
+  symmetry.
+  apply nonneg_L_elem.
+}
+rewrite first_coef. rewrite second_coef.
+apply tensor_decomp.
 Qed.
 
 Property is_unitary_form : forall (M : Square 2) (a b : Vector 2), 
@@ -39,12 +238,7 @@ Proof.
   rewrite qubit_adj_mult in WF_a. 2: apply H.
   rewrite qubit_adj_mult in WF_b. 2: apply H0.
   unfold WF_Unitary.
-  split. 
-  {
-    apply WF_plus.
-    apply WF_kron. reflexivity. reflexivity. apply H. apply WF_adjoint. apply WF_qubit0.
-    apply WF_kron. reflexivity. reflexivity. apply H0. apply WF_adjoint. apply WF_qubit1.
-  }
+  split. solve_WF_matrix.
   rewrite Mplus_adjoint.
   rewrite (kron_adjoint a ⟨0∣).
   rewrite (kron_adjoint b ⟨1∣).
@@ -100,14 +294,13 @@ assert (WF_Q : WF_Unitary Q).
   apply H2.
 }
 assert (HQ_impl := qubit_decomposition2 ((Q ⊗ I 2)† × w)).
-assert (WF_QI2 : WF_Matrix (Q ⊗ I 2)). 
+assert (WF_QI2 : WF_Matrix (Q ⊗ I 2)).
 {
-  apply WF_kron. reflexivity. reflexivity. apply WF_Q. apply WF_I.
+  solve_WF_matrix. apply H. apply H0.
 }
 assert (HQ: WF_Matrix ((Q ⊗ I 2) † × w)). 
 {
-  apply WF_mult. apply WF_adjoint. apply WF_QI2.
-  apply H1.
+  solve_WF_matrix. apply H. apply H0. apply H1.
 }
 apply HQ_impl in HQ.
 destruct HQ as [c00 [c01 [c10 [c11 HQ]]]].
@@ -119,25 +312,14 @@ rewrite <- ket0_equiv in HQ.
 rewrite <- ket1_equiv in HQ.
 set (psi := c00 .* ∣0⟩ .+ c01 .* ∣1⟩).
 set (phi := c10 .* ∣0⟩ .+ c11 .* ∣1⟩).
-assert (WF_psi: WF_Matrix psi).
-{
-  apply WF_plus. apply WF_scale. apply WF_qubit0. apply WF_scale. apply WF_qubit1.
-}
-assert (WF_phi: WF_Matrix phi).
-{
-  apply WF_plus. apply WF_scale. apply WF_qubit0. apply WF_scale. apply WF_qubit1.
-}
+assert (WF_psi: WF_Matrix psi). solve_WF_matrix.
+assert (WF_phi: WF_Matrix phi). solve_WF_matrix.
 fold psi in HQ. fold phi in HQ.
 exists psi, phi.
 assert (Step1: beta ⊗ psi .+ beta_p ⊗ phi = (Q ⊗ I 2) × (∣0⟩ ⊗ psi .+ ∣1⟩ ⊗ phi)).
 {
   lma'.
-  apply WF_plus. 
-  apply WF_kron. reflexivity. reflexivity. apply H.
-  apply WF_psi.
-  apply WF_kron. reflexivity. reflexivity. apply H0.
-  apply WF_phi.
-
+  solve_WF_matrix. apply H. apply H0.
 }
 rewrite Step1.
 rewrite <- HQ.
@@ -159,3 +341,74 @@ Qed.
 Definition linearly_independent_2vec {n} (v1 v2 : Vector n) := 
   forall (c1 c2 : C), c1 .* v1 .+ c2 .* v2 = Zero -> c1 = 0 /\ c2=0.
 
+Lemma addition_equivalence: forall (a b c: C), 
+a + b = c <-> b = c - a.
+Proof.
+split.
+intros.
+rewrite <- H.
+lca.
+intros.
+rewrite H.
+lca.
+Qed.
+
+Lemma opp_equivalence: forall (a b: C), 
+a = b <-> -a = -b.
+Proof.
+split.
+intros.
+rewrite H. reflexivity.
+intros.
+rewrite <- Cplus_0_l.
+rewrite <- (Cplus_opp_l a).
+rewrite H.
+lca.
+Qed.
+
+(* Lemma inner_prod_adj *)
+
+(* Using old version of proof since beta is chosen constructively *)
+(* Lemma a16_part1: forall (w0 w1 a0 a1 : Vector 2), 
+WF_Qubit a0 -> WF_Qubit a1 -> linearly_independent_2vec a0 a1 -> 
+w0 ⊗ a0 .+ w1 ⊗ a1 = Zero -> w0 = Zero.
+Proof.
+intros.
+set (beta := a1 .+ -⟨a0, a1⟩ .* a0).
+assert (Step1: ⟨beta, a0⟩ = 0).
+{
+  unfold beta, inner_product.
+  rewrite Mplus_adjoint.
+  rewrite Mmult_plus_distr_r.
+  rewrite Mscale_adj.
+  destruct H as [_ [WF_a0 H]].
+  rewrite qubit_adj_mult in H. 2: apply WF_a0.
+  rewrite Mscale_mult_dist_l.
+  rewrite H.
+  lca.
+}
+assert (Step2: ⟨beta, a1⟩ <> 0).
+{
+  unfold beta, inner_product.
+  rewrite Mplus_adjoint.
+  rewrite Mmult_plus_distr_r.
+  destruct H0 as [_ [WF_a1 H0]].
+  rewrite qubit_adj_mult in H0. 2: apply WF_a1.
+  rewrite H0.
+  rewrite Mscale_adj.
+  rewrite Mscale_mult_dist_l.
+  unfold Mplus. unfold I. simpl.
+  unfold scale.
+  fold (inner_product a0 a1).
+  rewrite Cconj_opp. rewrite <- Copp_mult_distr_l.
+  unfold not.
+  rewrite addition_equivalence.
+  rewrite Cminus_unfold.
+  rewrite Cplus_0_l.
+  rewrite <- opp_equivalence.
+  assert (⟨ a0, a1 ⟩ = ((a0 0%nat 0%nat)^* * (a1 0%nat 0%nat) + (a0 1%nat 0%nat)^* * (a1 1%nat 0%nat))). lca.
+  rewrite H3.
+  rewrite Cconj_plus_distr. rewrite Cconj_mult_distr. rewrite Cconj_involutive.
+  rewrite Cmult_plus_distr_l. rewrite Cmult_plus_distr_r. rewrite Cmult_plus_distr_r.
+  intros. 
+} *)
